src/SoftBound/sb_ds_pp.v
@@ -1630,16 +1630,16 @@ Proof.
   intros TD gl vc gv bc ec J1 J2.  
   remember (_const2GV TD gl vc) as J3.
   destruct J3 as [[gv3 t3]|]; inv J1.
-  generalize dependent gv.
+  generalize dependent gv3.
   generalize dependent t3.
   generalize dependent ec.
   generalize dependent bc.
   induction vc; intros; try solve [inversion J2].
-    exists gv. 
+    exists (? gv3 # t3 ?). 
     remember t as T.
     destruct T; inversion J2; clear J2; subst bc ec; simpl in *; 
     unfold mbitcast, p8; try solve [
-      destruct (lookupAL GenericValue gl i0); inversion HeqJ3; subst gv t3;
+      destruct (lookupAL GenericValue gl i0); inversion HeqJ3; subst gv3 t3;
       destruct (GV2ptr TD (getPointerSize TD) g); eauto;
       remember (mgep TD t v 
         (INTEGER.to_Z (INTEGER.of_Z 32 1 false) :: nil)) as optr;
@@ -1654,12 +1654,12 @@ Proof.
     destruct R as [[gv2 t2]|]; try solve [inv HeqJ3].
     destruct (mcast TD castop_bitcast t2 (typ_pointer t) gv2); 
       try solve [inv HeqJ3].
-    apply IHvc with (gv:=gv2)(t3:=t2) in H0; auto.
+    apply IHvc with (gv3:=gv2)(t3:=t2) in H0; auto.
     
     simpl in *.
     remember (_const2GV TD gl vc) as R.
     destruct R as [[gv2 t2]|]; try solve [inv HeqJ3].
-    apply IHvc with (gv:=gv2)(t3:=t2) in J2; auto.
+    apply IHvc with (gv3:=gv2)(t3:=t2) in J2; auto.
 Qed.
 
 Lemma wf_phinodes__getIncomingValuesForBlockFromPHINodes : forall
